functorized name overlays, failure recorder, and aggregation

core/NameOverlay.v
@@ -5,123 +5,143 @@ Require Import StructTact.Fin.
 Require Import mathcomp.ssreflect.ssreflect.
 Require Import mathcomp.ssreflect.ssrbool.
 
-Require Import MSetList.
-Require Import FMapList.
+Require Import OrderedType.
 
-Module Adjacency (N : NatValue).
+Module Type NameType.
+Parameter name : Type.
+Parameter name_eq_dec : forall x y : name, {x = y} + {x <> y}.
+Parameter nodes : list name.
+Parameter all_names_nodes : forall n, In n nodes.
+Parameter no_dup_nodes : NoDup nodes.
+End NameType.
 
-Module fin_n_OT := fin_OT N.
-Module FinNSet <: MSetInterface.S := MSetList.Make fin_n_OT.
-Definition FinNS := FinNSet.t.
+Module Type AdjacentNameType (Import NT : NameType).
+Parameter adjacent_to : relation name.
+Parameter adjacent_to_dec : forall x y : name, {adjacent_to x y} + {~ adjacent_to x y}.
+Parameter adjacent_to_symmetric : Symmetric adjacent_to.
+Parameter adjacent_to_irreflexive : Irreflexive adjacent_to.
+End AdjacentNameType.
 
-Module fin_n_OT_compat := fin_OT_compat N.
-Module FinNMap <: FMapInterface.S := FMapList.Make fin_n_OT_compat.
+Module Type NameOrderedTypeCompat (Import NT : NameType) <: OrderedType.
+Definition t := name.
+Definition eq := eq (A := name).
+Parameter lt : name -> name -> Prop.
+Definition eq_refl := eq_refl (A := name).
+Definition eq_sym := eq_sym (A := name).
+Definition eq_trans := eq_trans (A := name).
+Parameter lt_trans : forall x y z : t, lt x y -> lt y z -> lt x z.
+Parameter lt_not_eq : forall x y : t, lt x y -> ~ eq x y.
+Parameter compare : forall x y : t, Compare lt eq x y.
+Definition eq_dec := name_eq_dec.
+End NameOrderedTypeCompat.
 
-Instance Fin_n_NameParams : NameParams :=
-  { 
-    name := fin N.n ;
-    name_eq_dec := fin_eq_dec N.n ;
-    nodes := all_fin N.n ;
-    all_names_nodes := all_fin_all N.n ;
-    no_dup_nodes := all_fin_NoDup N.n
-  }.
+Require Import MSetInterface.
 
-Section Adjacent.
+Module Type NameOrderedType (Import NT : NameType) <: OrderedType.
+Definition t := name.
+Definition eq := eq (A := name).
+Definition eq_equiv := eq_equivalence (A := name).
+Parameter lt : name -> name -> Prop.
+Parameter lt_strorder : StrictOrder lt.
+Parameter lt_compat : Proper (eq==>eq==>iff) lt.
+Parameter compare : forall x y : name, comparison.
+Parameter compare_spec : forall x y, CompSpec eq lt x y (compare x y).
+Definition eq_dec := name_eq_dec.
+End NameOrderedType.
 
-  Context {fin_nop : NameOverlayParams Fin_n_NameParams}.
+Module Adjacency (Import NT : NameType) (Import ANT : AdjacentNameType NT) (NOT : NameOrderedType NT) (NSet : MSetInterface.S with Module E := NOT).
 
-  Definition adjacent_to_node (n : name) := 
-  filter (adjacent_to_dec n).
+Definition NS := NSet.t.
 
-  Lemma adjacent_to_node_adjacent_to : 
+Definition adjacent_to_node (n : name) := filter (adjacent_to_dec n).
+
+Lemma adjacent_to_node_adjacent_to : 
   forall n n' ns,
   In n' (adjacent_to_node n ns) -> In n' ns /\ adjacent_to n n'.
-  Proof.
-  move => n n' ns H_in.
-  rewrite /adjacent_to_node in H_in.
-  apply filter_In in H_in.
-  move: H_in => [H_in H_eq].
-  split => //.
-  move: H_eq.
-  by case adjacent_to_dec.
-  Qed.
+Proof.
+move => n n' ns H_in.
+rewrite /adjacent_to_node in H_in.
+apply filter_In in H_in.
+move: H_in => [H_in H_eq].
+split => //.
+move: H_eq.
+by case adjacent_to_dec.
+Qed.
 
-  Lemma adjacent_to_adjacent_to_node : 
-    forall n n' ns,
-      In n' ns -> 
-      adjacent_to n n' ->
-      In n' (adjacent_to_node n ns).
-  Proof.
-  move => n n' ns H_in H_adj.
-  apply filter_In.
-  split => //.
-  by case adjacent_to_dec.
-  Qed.
+Lemma adjacent_to_adjacent_to_node : 
+  forall n n' ns,
+    In n' ns -> 
+    adjacent_to n n' ->
+    In n' (adjacent_to_node n ns).
+Proof.
+move => n n' ns H_in H_adj.
+apply filter_In.
+split => //.
+by case adjacent_to_dec.
+Qed.
 
-  Definition adjacency (n : name) (ns : list name) : FinNS :=
-  fold_right (fun n' fs => FinNSet.add n' fs) FinNSet.empty (adjacent_to_node n ns).
+Definition adjacency (n : name) (ns : list name) : NS :=
+  fold_right (fun n' fs => NSet.add n' fs) NSet.empty (adjacent_to_node n ns).
 
-  Lemma adjacent_to_node_adjacency : 
-    forall n n' ns, 
-      In n' (adjacent_to_node n ns) <-> FinNSet.In n' (adjacency n ns).
-  Proof.
-  move => n n' ns.
-  split.
-  elim: ns => //=.
-  move => n0 ns IH.
-  rewrite /adjacency /= /is_left.
-  case adjacent_to_dec => H_dec /= H_in; last exact: IH.
-  case: H_in => H_in.
-    rewrite H_in.
-    apply FinNSet.add_spec.
-    by left.
-  apply FinNSet.add_spec.
-  right.
-  exact: IH.
-  elim: ns => //=; first by rewrite /adjacency /=; exact: FinNSet.empty_spec.
-  move => n0 ns IH.
-  rewrite /adjacency /=.
-  rewrite /is_left.
-  case adjacent_to_dec => H_dec /= H_ins; last exact: IH.
-  apply FinNSet.add_spec in H_ins.
-  case: H_ins => H_ins; first by left.
-  right.
-  exact: IH.
-  Qed.
+Lemma adjacent_to_node_adjacency : 
+  forall n n' ns, 
+    In n' (adjacent_to_node n ns) <-> NSet.In n' (adjacency n ns).
+Proof.
+move => n n' ns.
+split.
+elim: ns => //=.
+move => n0 ns IH.
+rewrite /adjacency /= /is_left.
+case adjacent_to_dec => H_dec /= H_in; last exact: IH.
+case: H_in => H_in.
+  rewrite H_in.
+  apply NSet.add_spec.
+  by left.
+apply NSet.add_spec.
+right.
+exact: IH.
+elim: ns => //=; first by rewrite /adjacency /=; exact: NSet.empty_spec.
+move => n0 ns IH.
+rewrite /adjacency /=.
+rewrite /is_left.
+case adjacent_to_dec => H_dec /= H_ins; last exact: IH.
+apply NSet.add_spec in H_ins.
+case: H_ins => H_ins; first by left.
+right.
+exact: IH.
+Qed.
 
-  Lemma not_adjacent_self : 
-    forall n ns, ~ FinNSet.In n (adjacency n ns).
-  Proof.
-  move => n ns H_ins.
-  apply adjacent_to_node_adjacency in H_ins.
-  apply adjacent_to_node_adjacent_to in H_ins.
-  move: H_ins => [H_in H_adj].
-  contradict H_adj.
-  exact: adjacent_to_irreflexive.
-  Qed.
+Lemma not_adjacent_self : 
+  forall n ns, ~ NSet.In n (adjacency n ns).
+Proof.
+move => n ns H_ins.
+apply adjacent_to_node_adjacency in H_ins.
+apply adjacent_to_node_adjacent_to in H_ins.
+move: H_ins => [H_in H_adj].
+contradict H_adj.
+exact: adjacent_to_irreflexive.
+Qed.
 
-  Lemma adjacency_mutual_in : 
-    forall n n' ns,
-    In n' ns ->
-    FinNSet.In n (adjacency n' ns) -> 
-    FinNSet.In n' (adjacency n ns).
-  Proof.
-  move => n n' ns H_in H_ins.
-  apply adjacent_to_node_adjacency.
-  apply adjacent_to_node_adjacency in H_ins.
-  apply adjacent_to_node_adjacent_to in H_ins.
-  move: H_ins => [H_in' H_adj].
-  apply adjacent_to_symmetric in H_adj.
-  exact: adjacent_to_adjacent_to_node.
-  Qed.
+Lemma adjacency_mutual_in : 
+  forall n n' ns,
+  In n' ns ->
+  NSet.In n (adjacency n' ns) -> 
+  NSet.In n' (adjacency n ns).
+Proof.
+move => n n' ns H_in H_ins.
+apply adjacent_to_node_adjacency.
+apply adjacent_to_node_adjacency in H_ins.
+apply adjacent_to_node_adjacent_to in H_ins.
+move: H_ins => [H_in' H_adj].
+apply adjacent_to_symmetric in H_adj.
+exact: adjacent_to_adjacent_to_node.
+Qed.
 
-  Lemma adjacency_mutual : forall (n n' : name), FinNSet.In n (adjacency n' nodes) -> FinNSet.In n' (adjacency n nodes).
-  Proof.
-  move => n n' H_ins.
-  have H_in: In n' nodes by exact: all_names_nodes.
-  exact: adjacency_mutual_in.
-  Qed.
-
-End Adjacent.
+Lemma adjacency_mutual : forall (n n' : name), NSet.In n (adjacency n' nodes) -> NSet.In n' (adjacency n nodes).
+Proof.
+move => n n' H_ins.
+have H_in: In n' nodes by exact: all_names_nodes.
+exact: adjacency_mutual_in.
+Qed.
 
 End Adjacency.
